\documentclass[titlepage]{article}

\usepackage{amsmath}
\usepackage{amssymb}
\usepackage{fullpage}

\DeclareMathOperator{\arccot}{arccot}

\title{Assignment 2}
\date{\today}
\author{Jerry Jiang\\ TianQi Shi}

\begin{document}
\maketitle

\noindent
\section{Problem Set 1}
\subsection{Problem 1}
a) $y' + 3x^2y^2 = 0, y(0) = 1$
\begin{align*}
  & y' + 3x^2y^2 = 0, y(0) = 1
  \\ & y' = -3x^2y^2
  \\ & \frac{dy}{dx} = -3x^2y^2
  \\ & \frac{dy}{y^2} = -3x^2 dx
  \\ \int & \frac{dy}{y^2} = \int -3x^2 dx
  \\ & \frac{-1}{y} = -x^3 + C
  \\ & -1 = (-x^3 + C)y
  \\ & y = \frac{-1}{-x^3 + C}
\end{align*}

Particular solution:

\begin{align*}
  & y = \frac{-1}{-x^3 + C}
  \\ & 1 = \frac{-1}{0 + C}
  \\ & 1 = \frac{-1}{C}
  \\ & C = -1
\end{align*}

$$\therefore y = \frac{-1}{-x^3 - 1} = \frac{1}{x^3 + 1}$$


\noindent
b) $x^2y' = 1 + y^2$

\begin{align*}
  & x^2y' = 1 + y^2
  \\ & \frac{dyx^2}{dx} = 1 + y^2
  \\ & \frac{dy}{1 + y^2} = \frac{1}{x^2} dx
  \\ \int & \frac{dy}{1 + y^2} = \int \frac{1}{x^2} dx
  \\ & \arctan y = \frac{-1}{x} + C
  \\ & y = \tan(\frac{-1}{x} + C) \end{align*}

\subsection{Problem 2}

\begin{align*}
  & (x-1)y' + \frac{2(x-1)y}{x} = (x-1)(x+1)
  \\ & y' + \frac{2y}{x} = x+1 \tag{$x \neq 1$}
  \\ & \sigma y' + \sigma \frac{2y}{x} = \sigma(x+1)
\end{align*}

Use integrating factor method:

\begin{align*}
  & (\sigma y)' = \sigma y' + \sigma' y = \sigma y' + \sigma \frac{2y}{x}
  \\ & \sigma' y = \sigma \frac{2y}{x}
  \\ & \sigma' = \sigma \frac{2}{x}
  \\ & \frac{d\sigma}{dx} = \sigma \frac{2}{x}
  \\ & \frac{d\sigma}{\sigma} = \frac{2}{x} dx
  \\ \int & \frac{d\sigma}{\sigma} = \int \frac{2}{x} dx
  \\ & \ln|\sigma| = 2 \ln|x| + C
  \\ & |\sigma| = e^C|x|^2 \tag{$x \neq 0$}
  \\ & \sigma = Dx^2
\end{align*}

Calculate $y$:

\begin{align*}
  & \frac{dDx^2y}{dx} = Dx^2(x+1)
  \\ & \frac{dx^2y}{dx} = x^2(x+1)
  \\ & dx^2y = x^2(x+1) dx
  \\ & dx^2y = x^3 + x^2 dx
  \\ \int & dx^2y = \int x^3 + x^2 dx
  \\ & x^2y = \frac{x^4}{4} + \frac{x^3}{3} + C
  \\ & y = \frac{x^2}{4} + \frac{x}{3} + \frac{C}{x^2} \tag{$x \neq 0 $}
\end{align*}

In addition, $x \neq 1$, since we divided the original equation by $(x-1)$.

Find particular solution:

\begin{align*}
  & y = \frac{x^2}{4} + \frac{x}{3} + \frac{C}{x^2}
  \\ & \frac{7}{3} = \frac{2^2}{4} + \frac{2}{3} + \frac{C}{2^2}
  \\ & \frac{7}{3} = 1 + \frac{2}{3} + \frac{C}{4}
  \\ & \frac{7}{3} = \frac{5}{3} + \frac{C}{4}
  \\ & \frac{2}{3} = \frac{C}{4}
  \\ & \frac{8}{3} = C
\end{align*}

$$\therefore y = \frac{x^2}{4} + \frac{x}{3} + \frac{8}{3x^2}$$

\section{Problem Set 2}
\subsection{Problem 1}
Given the linear equation $xy' - y = x - 1$, solve for $y(x)$.
\\ a) $y(e) = 1$
\\ \\ Using the integrating factor method, first multiply all terms by the integrating factor $\sigma$:
\begin{align*}
xy' - y &= x - 1
\\ y' - \frac{y}{x} &= 1 - \frac{1}{x}
\\ \sigma y' - \sigma \frac{y}{x} &= \sigma - \sigma \frac{1}{x}
\end{align*}
Set the left hand side to $(\sigma y)'$:
\begin{align*}
(\sigma y)' &= \sigma y' - \sigma \frac{y}{x}
\\ \sigma y' + \sigma'y &= \sigma y' - \sigma \frac{y}{x}
\\ \sigma'y &= - \sigma \frac{y}{x}
\\ \frac{d\sigma}{dx} &= - \frac{\sigma}{x}
\\ \frac{d\sigma}{\sigma} &= - \frac{dx}{x}
\\ \ln \left| \sigma \right| &= - \ln \left| x \right|
\\ \sigma &= \frac{1}{x}
\end{align*}
Then set the right hand side to $\frac{d}{dx} (\sigma y)$:
\begin{align*}
\frac{d}{dx} (\frac{y}{x}) &= \frac{1}{x} - \frac{1}{x}\frac{1}{x}
\\ \int d (\frac{y}{x}) &= \int \frac{1}{x} - \frac{1}{x^2} dx
\\ \frac{y}{x} &= \ln \left| x \right| + \frac{1}{x} + c
\\ y &= x\ln \left| x \right| + cx + 1
\end{align*}
Substituting initial conditions,
\begin{align*}
1 &= e\ln \left| e \right| + ce + 1
\\ 0 &= (c + 1)e
\\ c &= - 1
\end{align*}
$$ \therefore y = x\ln \left| x \right| - x + 1 $$

\noindent
b) $y (-1) = 1$
\\ Using the same general solution, substitute initial conditions.
\begin{align*}
1 &= (-1)\ln \left| (-1) \right| + c(-1) + 1
\\ c &= 0
\end{align*}
$$ \therefore y = x\ln \left| x \right| + 1 $$

\noindent
c) $y (0) = 1$
\\ The general solution contains a term $\ln \left| x \right|$ and the natural logarithm is indeterminate at $x=0$. Therefore, there is no particular solution satisfying this initial condition.


\subsection{Problem 2}
Solve for $y(x)$ given initial condition y(0) = -2:
\begin{align*}
y' &= \frac{e^x}{2y}
\\ \frac{dy}{dx} &= \frac{e^x}{2y}
\\ \int 2y dy &= \int e^x dx
\\ y^2 &= e^x + c
\\ y &= e^{\frac{x}{2}} + c
\end{align*}
Substituting initial conditions,
\begin{align*}
-2 &= e^{\frac{0}{2}} + c
\\ c &= -2
\end{align*}
Thus $y(x) = e^{\frac{x}{2}} - 2$

\end{document}
