\documentclass[titlepage]{article}
\usepackage{amsmath}
\usepackage{amssymb}
\usepackage{fullpage}
\usepackage{graphicx}

\DeclareMathOperator{\arccot}{arccot}

\title{Assignment 5}
\date{\today}
\author{Jerry Jiang\\ TianQi Shi}

\begin{document}
\maketitle

\noindent
\section{Problem Set 1}
\subsection{Problem 1}
1) $f(t) = e^{2^{t^2}}$ \\
This function is not exponential order. For some $K, c, T$,
$$\frac{e^{2^{t^2}}}{Ke^{ct}} = \frac{1}{K}e^{2^{t^2} - ct}$$
As $t$ approaches infinity, the expression in the exponent approaches infinity regardless of our selection of c.\\

\noindent 2) $f(t) = 2t^3$ \\
$$\lim_{t\to\infty} \frac{2t^3}{Ke^{ct}} = \lim_{t\to\infty} \frac{6t^2}{cKe^{ct}} = \lim_{t\to\infty} \frac{12t}{c^2Ke^{ct}} = \lim_{t\to\infty} \frac{12}{c^3Ke^{ct}}$$
Evaluating this limit, we see that as $t$ approaches infinity, the ratio approaches zero. Therefore $2t^3$ is of exponential order. Pick $K=100, c = 1, T = 1$.

\subsection{Problem 2}
$$F(s) = \frac{1}{s^2 + 6s + 8}$$

Using partial fraction decomposition,
\begin{align*}
  \frac{1}{s^2 + 6s + 8} &= \frac{A}{s+2} + \frac{B}{s+4} \\
  1 &= As + 4A + Bs + 2B \\
\end{align*}
Comparing coefficients,
\begin{align*}
  0 &= A + B \\
  1 &= 4A + 2B
\end{align*}
We get $A = 1/2$ and $B = -1/2$. Substituting,
$$F(s) = \frac{1}{s^2 + 6s + 8} = \frac{1}{2(s+2)} + \frac{-1}{2(s+4)}$$

Taking the inverse Laplace transform,
$$f(t) = \frac{1}{2}e^{-2t} - \frac{1}{2}e^{-4t}$$

\section{Problem Set 2}
\subsection{Problem 1}
$$y'' + 5y' + 4y = 0, y(0) = 1, y'(0) = 2$$
First we take the Laplace of both sides.
\begin{align*}
  &s^2Y(s) - sy(0) - y'(0) + 5(sY(s) - y(0)) + 4Y(s) = 0
  \\&s^2Y(s) - sy(0) - y'(0) + 5sY(s) - 5y(0) + 4Y(s) = 0
  \\&s^2Y(s) - s - 2 + 5sY(s) - 5 + 4Y(s) = 0
  \\&s^2Y(s) + 5sY(s) + 4Y(s) = s + 7
  \\&(s^2 + 5s + 4)Y(s) = s + 7
  \\&Y(s) = \frac{s + 7}{s^2  + 5s + 4}
  \\&Y(s) = \frac{s + 7}{(s + 1)(s + 4)}
\end{align*}
Use partial fraction decomposition to split $Y(s)$.
\begin{align*}
  &\frac{s + 7}{(s + 1)(s + 4)} = \frac{A}{s + 1} + \frac{B}{s + 4}
  \\& s + 7 = As + 4A + Bs + B
  \\&\therefore A + B = 1, 4A + B = 7
  \\&\therefore A = 2, B = -1
\end{align*}
Take the inverse Laplace to find $y(t)$.
\begin{align*}
  &Y(s) = \frac{s + 7}{(s + 1)(s + 4)}
  \\&Y(s) = \frac{2}{s + 1} - \frac{1}{s + 4}
  \\&y(t) = 2e^{-t} + e^{-4t}
\end{align*}
Therefore, the particular solution is $y(t) = 2e^{-t} + e^{-4t}$.

\subsection{Problem 2}
$$x'' + 7x' + 12x = 2 + e^{-t}, x(0) = 0, x'(0) = 1$$
First we take the Laplace of both sides.
\begin{align*}
  &s^2X(s) - sx(0) - x'(0) + 7sX(s) - 7x(0) + 12X(s) = \frac{2}{s} + \frac{1}{s + 1}
  \\&(s^2 + 7s + 12)X(s) = \frac{2}{s} + \frac{1}{s + 1} + 1
  \\&(s + 4)(s + 3)X(s) = \frac{2}{s} + \frac{1}{s + 1} + 1
  \\&X(s) = \frac{2}{s(s + 4)(s + 3)} + \frac{1}{(s + 1)(s + 4)(s + 3)} + \frac{1}{(s + 4)(s + 3)}
\end{align*}
Use partial fraction decomposition to split $X(s)$.
\begin{align*}
  &\frac{2}{s(s + 4)(s + 3)} = \frac{A}{s} + \frac{B}{s + 4} + \frac{C}{s + 3}
  \\&2 = As^2 + 7As + 12A + Bs^2 + 3Bs + Cs^2 + 4Cs
  \\&A + B + C = 0, 7A + 3B + 4C = 0, 12A = 2
  \\&A = \frac{1}{6}, B = \frac{1}{2}, C = -\frac{2}{3}
\end{align*}

\begin{align*}
  &\frac{1}{(s + 1)(s + 4)(s + 3)} = \frac{A}{s + 1} + \frac{B}{s + 4} + \frac{C}{s + 3}
  \\&1 = As^2 + 7As + 12A + Bs^2 + 4Bs + 3B + Cs^2 + 5Cs + 4C
  \\&A + B + C = 0, 7A + 4B + 5C = 0, 12A + 3B + 4C = 1
  \\&A = \frac{1}{6}, B = \frac{1}{3}, C = -\frac{1}{2}
\end{align*}

\begin{align*}
  &\frac{1}{(s + 4)(s + 3)} = \frac{A}{s + 4} + \frac{B}{s + 3}
  \\&1 = As + 3A + Bs + 4B
  \\&A + B = 0, 3A + 4B = 1
  \\&A = -1, B = 1
\end{align*}
Take the inverse Laplace to find $x(t)$.
\begin{align*}
  &X(s) = \frac{1}{6}\frac{1}{s} + \frac{1}{2}\frac{1}{s + 4} - \frac{2}{3}\frac{1}{s + 3} + \frac{1}{6}\frac{1}{s + 1} + \frac{1}{3}\frac{1}{s + 4} - \frac{1}{2}\frac{1}{s + 3} - \frac{1}{s + 4} + \frac{1}{s + 3}
  \\&X(s) = \frac{1}{6}\frac{1}{s} - \frac{1}{6}\frac{1}{s + 4} - \frac{1}{6}\frac{1}{s + 3} + \frac{1}{6}\frac{1}{s + 1}
  \\&x(t) = \frac{1}{6} - \frac{1}{6}e^{-4t} - \frac{1}{6}e^{-3t} + \frac{1}{6}e^{-t}
\end{align*}

Therefore, the particular solution is $x(t) = \frac{1}{6} - \frac{1}{6}e^{-4t} - \frac{1}{6}e^{-3t} + \frac{1}{6}e^{-t}$.

\end{document}
